Centro in $x_{0}=0$ 
1) $$(T^{n}e^{x}) = \sum\limits_{k=0}^{n} \frac{x^{k}}{k!} = 1 + x + \frac{x^{2}}{2} +\frac{x^{3}}{6}+\ldots+\frac{x^{n}}{n!}$$
2) $$(T^{n}log(1+x))=\sum\limits_{k=1}^{n}  \frac{(-1)^{k+1} \cdot x^{k}}{k}= x - \frac{x^{2}}{2}+\frac{x^{3}}{3}-\frac{x^{4}}{4} \ldots $$
3) $$(T^{2n+1}sinx)=\sum\limits_{k=0}^{n} \frac{(-1)^{k} \cdot x^{2k+1}}{(2k+1)!} = x -\frac{x^{3}}{6}+\frac{x^{5}}{5!} \ldots$$
4) $$(T^{2n}cosx) = \sum\limits_{k=0}^{n} \frac{(-1)^{k}\cdot x^{2k}}{(2k)!} = 1-\frac{x^{2}}{2}+\frac{x^{4}}{24}\ldots  $$
5) $$(T^{n}(1+x)^{\alpha})= 1 +\alpha x+\frac{\alpha(\alpha-1)}{2}x^{2}+\ldots +\begin{pmatrix} \alpha  \\ n \end{pmatrix}x^{n}$$
NB: $$\begin{pmatrix} \alpha  \\ n \end{pmatrix} = \frac{\alpha(\alpha-1)(\alpha-2)\ldots (\alpha+1-n)}{n!}$$
se $\alpha = k\in N$ allora:$$\begin{pmatrix} \alpha  \\ n \end{pmatrix} = \begin{pmatrix} k  \\ n \end{pmatrix} = \frac{k!}{(n-k)!n!}$$

Argomento principale: [[Calcolo Differenziale]]
Vedi: [[Polinomi di Taylor]]
#analisi1